src/generated.c
@@ -123,6 +123,10 @@ extern unsigned long long eval_ins(int);
 
 extern _Bool cmp_ptr32_nullM(unsigned char *);
 
+extern unsigned char *_bpf_get_call(int);
+
+extern unsigned int exec_function(unsigned char *);
+
 struct memory_region *get_mem_region(unsigned int n, struct memory_region *mrs)
 {
   return mrs + n;
@@ -138,63 +142,63 @@ unsigned int reg64_to_reg32(unsigned long long d)
   return (unsigned int) d;
 }
 
-unsigned int get_src(unsigned long long ins$116)
+unsigned int get_src(unsigned long long ins$120)
 {
-  return (unsigned int) ((ins$116 & 65535LLU) >> 12LLU);
+  return (unsigned int) ((ins$120 & 65535LLU) >> 12LLU);
 }
 
-int get_offset(unsigned long long ins$118)
+int get_offset(unsigned long long ins$122)
 {
-  return (int) (short) (ins$118 << 32LLU >> 48LLU);
+  return (int) (short) (ins$122 << 32LLU >> 48LLU);
 }
 
-int get_immediate(unsigned long long ins$120)
+int get_immediate(unsigned long long ins$124)
 {
-  return (int) (ins$120 >> 32LLU);
+  return (int) (ins$124 >> 32LLU);
 }
 
-long long eval_immediate(int ins$122)
+long long eval_immediate(int ins$126)
 {
-  return (long long) ins$122;
+  return (long long) ins$126;
 }
 
-unsigned long long get_src64(unsigned char x, unsigned long long ins$126)
+unsigned long long get_src64(unsigned char x, unsigned long long ins$130)
 {
   int imm;
   long long imm64;
   unsigned int src;
   unsigned long long src64;
   if (0 == (x & 8)) {
-    imm = get_immediate(ins$126);
+    imm = get_immediate(ins$130);
     imm64 = eval_immediate(imm);
     return imm64;
   } else {
-    src = get_src(ins$126);
+    src = get_src(ins$130);
     src64 = eval_reg(src);
     return src64;
   }
 }
 
-unsigned int get_src32(unsigned char x$136, unsigned long long ins$138)
+unsigned int get_src32(unsigned char x$140, unsigned long long ins$142)
 {
-  int imm$140;
-  unsigned int src$142;
-  unsigned long long src64$144;
+  int imm$144;
+  unsigned int src$146;
+  unsigned long long src64$148;
   unsigned int src32;
-  if (0 == (x$136 & 8)) {
-    imm$140 = get_immediate(ins$138);
-    return imm$140;
+  if (0 == (x$140 & 8)) {
+    imm$144 = get_immediate(ins$142);
+    return imm$144;
   } else {
-    src$142 = get_src(ins$138);
-    src64$144 = eval_reg(src$142);
-    src32 = reg64_to_reg32(src64$144);
+    src$146 = get_src(ins$142);
+    src64$148 = eval_reg(src$146);
+    src32 = reg64_to_reg32(src64$148);
     return src32;
   }
 }
 
-unsigned char get_opcode_ins(unsigned long long ins$148)
+unsigned char get_opcode_ins(unsigned long long ins$152)
 {
-  return (unsigned char) (ins$148 & 255LLU);
+  return (unsigned char) (ins$152 & 255LLU);
 }
 
 unsigned char get_opcode_alu64(unsigned char op)
@@ -202,54 +206,54 @@ unsigned char get_opcode_alu64(unsigned char op)
   return (unsigned char) (op & 240);
 }
 
-unsigned char get_opcode_alu32(unsigned char op$152)
+unsigned char get_opcode_alu32(unsigned char op$156)
 {
-  return (unsigned char) (op$152 & 240);
+  return (unsigned char) (op$156 & 240);
 }
 
-unsigned char get_opcode_branch(unsigned char op$154)
+unsigned char get_opcode_branch(unsigned char op$158)
 {
-  return (unsigned char) (op$154 & 240);
+  return (unsigned char) (op$158 & 240);
 }
 
-unsigned char get_opcode_mem_ld_imm(unsigned char op$156)
-{
-  return (unsigned char) (op$156 & 255);
-}
-
-unsigned char get_opcode_mem_ld_reg(unsigned char op$158)
-{
-  return (unsigned char) (op$158 & 255);
-}
-
-unsigned char get_opcode_mem_st_imm(unsigned char op$160)
+unsigned char get_opcode_mem_ld_imm(unsigned char op$160)
 {
   return (unsigned char) (op$160 & 255);
 }
 
-unsigned char get_opcode_mem_st_reg(unsigned char op$162)
+unsigned char get_opcode_mem_ld_reg(unsigned char op$162)
 {
   return (unsigned char) (op$162 & 255);
 }
 
-unsigned char get_opcode(unsigned char op$164)
+unsigned char get_opcode_mem_st_imm(unsigned char op$164)
 {
-  return (unsigned char) (op$164 & 7);
+  return (unsigned char) (op$164 & 255);
 }
 
-unsigned int get_add(unsigned int x$166, unsigned int y)
+unsigned char get_opcode_mem_st_reg(unsigned char op$166)
 {
-  return x$166 + y;
+  return (unsigned char) (op$166 & 255);
 }
 
-unsigned int get_sub(unsigned int x$170, unsigned int y$172)
+unsigned char get_opcode(unsigned char op$168)
 {
-  return x$170 - y$172;
+  return (unsigned char) (op$168 & 7);
 }
 
-unsigned int get_addr_ofs(unsigned long long x$174, int ofs)
+unsigned int get_add(unsigned int x$170, unsigned int y)
 {
-  return (unsigned int) (x$174 + (unsigned long long) ofs);
+  return x$170 + y;
+}
+
+unsigned int get_sub(unsigned int x$174, unsigned int y$176)
+{
+  return x$174 - y$176;
+}
+
+unsigned int get_addr_ofs(unsigned long long x$178, int ofs)
+{
+  return (unsigned int) (x$178 + (unsigned long long) ofs);
 }
 
 unsigned int get_start_addr(struct memory_region *mr)
@@ -257,14 +261,14 @@ unsigned int get_start_addr(struct memory_region *mr)
   return (*mr).start_addr;
 }
 
-unsigned int get_block_size(struct memory_region *mr$180)
+unsigned int get_block_size(struct memory_region *mr$184)
 {
-  return (*mr$180).block_size;
+  return (*mr$184).block_size;
 }
 
-unsigned int get_block_perm(struct memory_region *mr$182)
+unsigned int get_block_perm(struct memory_region *mr$186)
 {
-  return (*mr$182).block_perm;
+  return (*mr$186).block_perm;
 }
 
 _Bool is_well_chunk_bool(unsigned int chunk)
@@ -284,7 +288,7 @@ _Bool is_well_chunk_bool(unsigned int chunk)
   }
 }
 
-unsigned char *check_mem_aux2(struct memory_region *mr$186, unsigned int perm, unsigned int addr, unsigned int chunk$192)
+unsigned char *check_mem_aux2(struct memory_region *mr$190, unsigned int perm, unsigned int addr, unsigned int chunk$196)
 {
   _Bool well_chunk;
   unsigned int start;
@@ -292,17 +296,17 @@ unsigned char *check_mem_aux2(struct memory_region *mr$186, unsigned int perm, u
   unsigned int mr_perm;
   unsigned int lo_ofs;
   unsigned int hi_ofs;
-  well_chunk = is_well_chunk_bool(chunk$192);
+  well_chunk = is_well_chunk_bool(chunk$196);
   if (well_chunk) {
-    start = get_start_addr(mr$186);
-    size = get_block_size(mr$186);
-    mr_perm = get_block_perm(mr$186);
+    start = get_start_addr(mr$190);
+    size = get_block_size(mr$190);
+    mr_perm = get_block_perm(mr$190);
     lo_ofs = get_sub(addr, start);
-    hi_ofs = get_add(lo_ofs, chunk$192);
+    hi_ofs = get_add(lo_ofs, chunk$196);
     if (hi_ofs < size
-          && (lo_ofs <= 4294967295U - chunk$192 && 0U == lo_ofs % chunk$192)
+          && (lo_ofs <= 4294967295U - chunk$196 && 0U == lo_ofs % chunk$196)
           && mr_perm >= perm) {
-      return (*mr$186).block_ptr + lo_ofs;
+      return (*mr$190).block_ptr + lo_ofs;
     } else {
       return 0;
     }
@@ -311,102 +315,102 @@ unsigned char *check_mem_aux2(struct memory_region *mr$186, unsigned int perm, u
   }
 }
 
-unsigned char *check_mem_aux(unsigned int num, unsigned int perm$208, unsigned int chunk$210, unsigned int addr$212, struct memory_region *mrs$214)
+unsigned char *check_mem_aux(unsigned int num, unsigned int perm$212, unsigned int chunk$214, unsigned int addr$216, struct memory_region *mrs$218)
 {
-  unsigned int n$216;
+  unsigned int n$220;
   struct memory_region *cur_mr;
-  unsigned char *check_mem$220;
+  unsigned char *check_mem$224;
   _Bool is_null;
   if (num == 0U) {
     return 0;
   } else {
-    n$216 = num - 1U;
-    cur_mr = get_mem_region(n$216, mrs$214);
-    check_mem$220 = check_mem_aux2(cur_mr, perm$208, addr$212, chunk$210);
-    is_null = cmp_ptr32_nullM(check_mem$220);
+    n$220 = num - 1U;
+    cur_mr = get_mem_region(n$220, mrs$218);
+    check_mem$224 = check_mem_aux2(cur_mr, perm$212, addr$216, chunk$214);
+    is_null = cmp_ptr32_nullM(check_mem$224);
     if (is_null) {
-      return check_mem_aux(n$216, perm$208, chunk$210, addr$212, mrs$214);
+      return check_mem_aux(n$220, perm$212, chunk$214, addr$216, mrs$218);
     } else {
-      return check_mem$220;
+      return check_mem$224;
     }
   }
 }
 
-unsigned char *check_mem(unsigned int perm$224, unsigned int chunk$226, unsigned int addr$228)
+unsigned char *check_mem(unsigned int perm$228, unsigned int chunk$230, unsigned int addr$232)
 {
-  _Bool well_chunk$230;
+  _Bool well_chunk$234;
   unsigned int mem_reg_num;
-  struct memory_region *mrs$234;
-  unsigned char *check_mem$236;
-  _Bool is_null$238;
-  well_chunk$230 = is_well_chunk_bool(chunk$226);
-  if (well_chunk$230) {
+  struct memory_region *mrs$238;
+  unsigned char *check_mem$240;
+  _Bool is_null$242;
+  well_chunk$234 = is_well_chunk_bool(chunk$230);
+  if (well_chunk$234) {
     mem_reg_num = eval_mrs_num();
-    mrs$234 = eval_mrs_regions();
-    check_mem$236 =
-      check_mem_aux(mem_reg_num, perm$224, chunk$226, addr$228, mrs$234);
-    is_null$238 = cmp_ptr32_nullM(check_mem$236);
-    if (is_null$238) {
+    mrs$238 = eval_mrs_regions();
+    check_mem$240 =
+      check_mem_aux(mem_reg_num, perm$228, chunk$230, addr$232, mrs$238);
+    is_null$242 = cmp_ptr32_nullM(check_mem$240);
+    if (is_null$242) {
       return 0;
     } else {
-      return check_mem$236;
+      return check_mem$240;
     }
   } else {
     return 0;
   }
 }
 
-void step_opcode_alu64(unsigned long long dst64, unsigned long long src64$242, unsigned int dst, unsigned char op$246)
+void step_opcode_alu64(unsigned long long dst64, unsigned long long src64$246, unsigned int dst, unsigned char op$250)
 {
   unsigned char opcode_alu64;
-  unsigned int src32$250;
-  unsigned int src32$252;
   unsigned int src32$254;
-  opcode_alu64 = get_opcode_alu64(op$246);
+  unsigned int src32$256;
+  unsigned int src32$258;
+  opcode_alu64 = get_opcode_alu64(op$250);
   switch (opcode_alu64) {
     case 0:
-      upd_reg(dst, dst64 + src64$242);
+      upd_reg(dst, dst64 + src64$246);
       return;
     case 16:
-      upd_reg(dst, dst64 - src64$242);
+      upd_reg(dst, dst64 - src64$246);
       return;
     case 32:
-      upd_reg(dst, dst64 * src64$242);
+      upd_reg(dst, dst64 * src64$246);
       return;
     case 48:
-      if (src64$242 != 0LLU) {
-        upd_reg(dst, dst64 / src64$242);
+      if (src64$246 != 0LLU) {
+        upd_reg(dst, dst64 / src64$246);
         return;
       } else {
         upd_flag(-9);
         return;
       }
     case 64:
-      upd_reg(dst, dst64 | src64$242);
+      upd_reg(dst, dst64 | src64$246);
       return;
     case 80:
-      upd_reg(dst, dst64 & src64$242);
+      upd_reg(dst, dst64 & src64$246);
       return;
     case 96:
-      src32$250 = reg64_to_reg32(src64$242);
-      if (src32$250 < 64U) {
-        upd_reg(dst, dst64 << src32$250);
+      src32$254 = reg64_to_reg32(src64$246);
+      if (src32$254 < 64U) {
+        upd_reg(dst, dst64 << src32$254);
         return;
       } else {
         upd_flag(-10);
         return;
       }
     case 112:
-      src32$252 = reg64_to_reg32(src64$242);
-      if (src32$252 < 64U) {
-        upd_reg(dst, dst64 >> src32$252);
+      src32$256 = reg64_to_reg32(src64$246);
+      if (src32$256 < 64U) {
+        upd_reg(dst, dst64 >> src32$256);
         return;
       } else {
         upd_flag(-10);
         return;
       }
     case 128:
-      if (op$246 == 135) {
+      if (op$250 == 135) {
         upd_reg(dst, -dst64);
         return;
       } else {
@@ -414,23 +418,23 @@ void step_opcode_alu64(unsigned long long dst64, unsigned long long src64$242, u
         return;
       }
     case 144:
-      if (src64$242 != 0LLU) {
-        upd_reg(dst, dst64 % src64$242);
+      if (src64$246 != 0LLU) {
+        upd_reg(dst, dst64 % src64$246);
         return;
       } else {
         upd_flag(-9);
         return;
       }
     case 160:
-      upd_reg(dst, dst64 ^ src64$242);
+      upd_reg(dst, dst64 ^ src64$246);
       return;
     case 176:
-      upd_reg(dst, src64$242);
+      upd_reg(dst, src64$246);
       return;
     case 192:
-      src32$254 = reg64_to_reg32(src64$242);
-      if (src32$254 < 64U) {
-        upd_reg(dst, (unsigned long long) ((long long) dst64 >> src32$254));
+      src32$258 = reg64_to_reg32(src64$246);
+      if (src32$258 < 64U) {
+        upd_reg(dst, (unsigned long long) ((long long) dst64 >> src32$258));
         return;
       } else {
         upd_flag(-10);
@@ -443,75 +447,75 @@ void step_opcode_alu64(unsigned long long dst64, unsigned long long src64$242, u
   }
 }
 
-void step_opcode_alu32(unsigned int dst32, unsigned int src32$258, unsigned int dst$260, unsigned char op$262)
+void step_opcode_alu32(unsigned int dst32, unsigned int src32$262, unsigned int dst$264, unsigned char op$266)
 {
   unsigned char opcode_alu32;
-  opcode_alu32 = get_opcode_alu32(op$262);
+  opcode_alu32 = get_opcode_alu32(op$266);
   switch (opcode_alu32) {
     case 0:
-      upd_reg(dst$260, (unsigned long long) (dst32 + src32$258));
+      upd_reg(dst$264, (unsigned long long) (dst32 + src32$262));
       return;
     case 16:
-      upd_reg(dst$260, (unsigned long long) (dst32 - src32$258));
+      upd_reg(dst$264, (unsigned long long) (dst32 - src32$262));
       return;
     case 32:
-      upd_reg(dst$260, (unsigned long long) (dst32 * src32$258));
+      upd_reg(dst$264, (unsigned long long) (dst32 * src32$262));
       return;
     case 48:
-      if (src32$258 != 0U) {
-        upd_reg(dst$260, (unsigned long long) (dst32 / src32$258));
+      if (src32$262 != 0U) {
+        upd_reg(dst$264, (unsigned long long) (dst32 / src32$262));
         return;
       } else {
         upd_flag(-9);
         return;
       }
     case 64:
-      upd_reg(dst$260, (unsigned long long) (dst32 | src32$258));
+      upd_reg(dst$264, (unsigned long long) (dst32 | src32$262));
       return;
     case 80:
-      upd_reg(dst$260, (unsigned long long) (dst32 & src32$258));
+      upd_reg(dst$264, (unsigned long long) (dst32 & src32$262));
       return;
     case 96:
-      if (src32$258 < 32U) {
-        upd_reg(dst$260, (unsigned long long) (dst32 << src32$258));
+      if (src32$262 < 32U) {
+        upd_reg(dst$264, (unsigned long long) (dst32 << src32$262));
         return;
       } else {
         upd_flag(-10);
         return;
       }
     case 112:
-      if (src32$258 < 32U) {
-        upd_reg(dst$260, (unsigned long long) (dst32 >> src32$258));
+      if (src32$262 < 32U) {
+        upd_reg(dst$264, (unsigned long long) (dst32 >> src32$262));
         return;
       } else {
         upd_flag(-10);
         return;
       }
     case 128:
-      if (op$262 == 132) {
-        upd_reg(dst$260, (unsigned long long) -dst32);
+      if (op$266 == 132) {
+        upd_reg(dst$264, (unsigned long long) -dst32);
         return;
       } else {
         upd_flag(-1);
         return;
       }
     case 144:
-      if (src32$258 != 0U) {
-        upd_reg(dst$260, (unsigned long long) (dst32 % src32$258));
+      if (src32$262 != 0U) {
+        upd_reg(dst$264, (unsigned long long) (dst32 % src32$262));
         return;
       } else {
         upd_flag(-9);
         return;
       }
     case 160:
-      upd_reg(dst$260, (unsigned long long) (dst32 ^ src32$258));
+      upd_reg(dst$264, (unsigned long long) (dst32 ^ src32$262));
       return;
     case 176:
-      upd_reg(dst$260, (unsigned long long) src32$258);
+      upd_reg(dst$264, (unsigned long long) src32$262);
       return;
     case 192:
-      if (src32$258 < 32U) {
-        upd_reg(dst$260, (unsigned long long) ((int) dst32 >> src32$258));
+      if (src32$262 < 32U) {
+        upd_reg(dst$264, (unsigned long long) ((int) dst32 >> src32$262));
         return;
       } else {
         upd_flag(-10);
@@ -524,98 +528,117 @@ void step_opcode_alu32(unsigned int dst32, unsigned int src32$258, unsigned int 
   }
 }
 
-void step_opcode_branch(unsigned long long dst64$266, unsigned long long src64$268, int pc, int ofs$272, unsigned char op$274)
+void step_opcode_branch(unsigned long long dst64$270, unsigned long long src64$272, int pc, int ofs$276, unsigned char op$278)
 {
   unsigned char opcode_jmp;
-  opcode_jmp = get_opcode_branch(op$274);
+  unsigned char *f_ptr;
+  _Bool is_null$284;
+  unsigned int res;
+  opcode_jmp = get_opcode_branch(op$278);
   switch (opcode_jmp) {
     case 0:
-      if (op$274 == 5) {
-        upd_pc(pc + ofs$272);
+      if (op$278 == 5) {
+        upd_pc(pc + ofs$276);
         return;
       } else {
         upd_flag(-1);
         return;
       }
     case 16:
-      if (dst64$266 == src64$268) {
-        upd_pc(pc + ofs$272);
+      if (dst64$270 == src64$272) {
+        upd_pc(pc + ofs$276);
         return;
       } else {
         return;
       }
     case 32:
-      if (dst64$266 > src64$268) {
-        upd_pc(pc + ofs$272);
+      if (dst64$270 > src64$272) {
+        upd_pc(pc + ofs$276);
         return;
       } else {
         return;
       }
     case 48:
-      if (dst64$266 >= src64$268) {
-        upd_pc(pc + ofs$272);
+      if (dst64$270 >= src64$272) {
+        upd_pc(pc + ofs$276);
         return;
       } else {
         return;
       }
     case 160:
-      if (dst64$266 < src64$268) {
-        upd_pc(pc + ofs$272);
+      if (dst64$270 < src64$272) {
+        upd_pc(pc + ofs$276);
         return;
       } else {
         return;
       }
     case 176:
-      if (dst64$266 <= src64$268) {
-        upd_pc(pc + ofs$272);
+      if (dst64$270 <= src64$272) {
+        upd_pc(pc + ofs$276);
         return;
       } else {
         return;
       }
     case 64:
-      if ((dst64$266 & src64$268) != 0LLU) {
-        upd_pc(pc + ofs$272);
+      if ((dst64$270 & src64$272) != 0LLU) {
+        upd_pc(pc + ofs$276);
         return;
       } else {
         return;
       }
     case 80:
-      if (dst64$266 != src64$268) {
-        upd_pc(pc + ofs$272);
+      if (dst64$270 != src64$272) {
+        upd_pc(pc + ofs$276);
         return;
       } else {
         return;
       }
     case 96:
-      if ((long long) dst64$266 > (long long) src64$268) {
-        upd_pc(pc + ofs$272);
+      if ((long long) dst64$270 > (long long) src64$272) {
+        upd_pc(pc + ofs$276);
         return;
       } else {
         return;
       }
     case 112:
-      if ((long long) dst64$266 >= (long long) src64$268) {
-        upd_pc(pc + ofs$272);
+      if ((long long) dst64$270 >= (long long) src64$272) {
+        upd_pc(pc + ofs$276);
         return;
       } else {
         return;
       }
     case 192:
-      if ((long long) dst64$266 < (long long) src64$268) {
-        upd_pc(pc + ofs$272);
+      if ((long long) dst64$270 < (long long) src64$272) {
+        upd_pc(pc + ofs$276);
         return;
       } else {
         return;
       }
     case 208:
-      if ((long long) dst64$266 <= (long long) src64$268) {
-        upd_pc(pc + ofs$272);
+      if ((long long) dst64$270 <= (long long) src64$272) {
+        upd_pc(pc + ofs$276);
         return;
       } else {
         return;
       }
+    case 128:
+      if (op$278 == 133) {
+        f_ptr = _bpf_get_call((int) src64$272);
+        is_null$284 = cmp_ptr32_nullM(f_ptr);
+        if (is_null$284) {
+          upd_flag(-4);
+          return;
+        } else {
+          res = exec_function(f_ptr);
+          upd_reg(0U, (unsigned long long) res);
+          return;
+        }
+      } else {
+        upd_flag(-1);
+        return;
+      }
     case 144:
-      if (op$274 == 149) {
+      if (op$278 == 149) {
         upd_flag(1);
         return;
       } else {
@@ -629,21 +652,21 @@ void step_opcode_branch(unsigned long long dst64$266, unsigned long long src64$2
   }
 }
 
-void step_opcode_mem_ld_imm(int imm$278, int pc$280, unsigned int dst$282, unsigned char op$284)
+void step_opcode_mem_ld_imm(int imm$288, int pc$290, unsigned int dst$292, unsigned char op$294)
 {
   int len;
   unsigned char opcode_ld;
   unsigned long long next_ins;
   int next_imm;
   len = eval_ins_len();
-  opcode_ld = get_opcode_mem_ld_imm(op$284);
+  opcode_ld = get_opcode_mem_ld_imm(op$294);
   switch (opcode_ld) {
     case 24:
-      if (pc$280 + 1 < len) {
-        next_ins = eval_ins(pc$280 + 1);
+      if (pc$290 + 1 < len) {
+        next_ins = eval_ins(pc$290 + 1);
         next_imm = get_immediate(next_ins);
-        upd_reg(dst$282,
-                (unsigned long long) imm$278
+        upd_reg(dst$292,
+                (unsigned long long) imm$288
                   | (unsigned long long) next_imm << 32U);
         upd_pc_incr();
         return;
@@ -658,65 +681,65 @@ void step_opcode_mem_ld_imm(int imm$278, int pc$280, unsigned int dst$282, unsig
   }
 }
 
-void step_opcode_mem_ld_reg(unsigned int addr$294, int pc$296, unsigned int dst$298, unsigned char op$300)
+void step_opcode_mem_ld_reg(unsigned int addr$304, int pc$306, unsigned int dst$308, unsigned char op$310)
 {
-  unsigned char opcode_ld$302;
+  unsigned char opcode_ld$312;
   unsigned char *addr_ptr;
-  _Bool is_null$306;
+  _Bool is_null$316;
   unsigned long long v;
-  unsigned char *addr_ptr$310;
-  _Bool is_null$312;
-  unsigned long long v$314;
-  unsigned char *addr_ptr$316;
-  _Bool is_null$318;
-  unsigned long long v$320;
-  unsigned char *addr_ptr$322;
-  _Bool is_null$324;
-  unsigned long long v$326;
-  opcode_ld$302 = get_opcode_mem_ld_reg(op$300);
-  switch (opcode_ld$302) {
+  unsigned char *addr_ptr$320;
+  _Bool is_null$322;
+  unsigned long long v$324;
+  unsigned char *addr_ptr$326;
+  _Bool is_null$328;
+  unsigned long long v$330;
+  unsigned char *addr_ptr$332;
+  _Bool is_null$334;
+  unsigned long long v$336;
+  opcode_ld$312 = get_opcode_mem_ld_reg(op$310);
+  switch (opcode_ld$312) {
     case 97:
-      addr_ptr = check_mem(1U, 4U, addr$294);
-      is_null$306 = cmp_ptr32_nullM(addr_ptr);
-      if (is_null$306) {
+      addr_ptr = check_mem(1U, 4U, addr$304);
+      is_null$316 = cmp_ptr32_nullM(addr_ptr);
+      if (is_null$316) {
         upd_flag(-2);
         return;
       } else {
         v = load_mem(4U, addr_ptr);
-        upd_reg(dst$298, v);
+        upd_reg(dst$308, v);
         return;
       }
     case 105:
-      addr_ptr$310 = check_mem(1U, 2U, addr$294);
-      is_null$312 = cmp_ptr32_nullM(addr_ptr$310);
-      if (is_null$312) {
+      addr_ptr$320 = check_mem(1U, 2U, addr$304);
+      is_null$322 = cmp_ptr32_nullM(addr_ptr$320);
+      if (is_null$322) {
         upd_flag(-2);
         return;
       } else {
-        v$314 = load_mem(2U, addr_ptr$310);
-        upd_reg(dst$298, v$314);
+        v$324 = load_mem(2U, addr_ptr$320);
+        upd_reg(dst$308, v$324);
         return;
       }
     case 113:
-      addr_ptr$316 = check_mem(1U, 1U, addr$294);
-      is_null$318 = cmp_ptr32_nullM(addr_ptr$316);
-      if (is_null$318) {
+      addr_ptr$326 = check_mem(1U, 1U, addr$304);
+      is_null$328 = cmp_ptr32_nullM(addr_ptr$326);
+      if (is_null$328) {
         upd_flag(-2);
         return;
       } else {
-        v$320 = load_mem(1U, addr_ptr$316);
-        upd_reg(dst$298, v$320);
+        v$330 = load_mem(1U, addr_ptr$326);
+        upd_reg(dst$308, v$330);
         return;
       }
     case 121:
-      addr_ptr$322 = check_mem(1U, 8U, addr$294);
-      is_null$324 = cmp_ptr32_nullM(addr_ptr$322);
-      if (is_null$324) {
+      addr_ptr$332 = check_mem(1U, 8U, addr$304);
+      is_null$334 = cmp_ptr32_nullM(addr_ptr$332);
+      if (is_null$334) {
         upd_flag(-2);
         return;
       } else {
-        v$326 = load_mem(8U, addr_ptr$322);
-        upd_reg(dst$298, v$326);
+        v$336 = load_mem(8U, addr_ptr$332);
+        upd_reg(dst$308, v$336);
         return;
       }
     default:
@@ -726,57 +749,57 @@ void step_opcode_mem_ld_reg(unsigned int addr$294, int pc$296, unsigned int dst$
   }
 }
 
-void step_opcode_mem_st_imm(int imm$328, unsigned int addr$330, int pc$332, unsigned int dst$334, unsigned char op$336)
+void step_opcode_mem_st_imm(int imm$338, unsigned int addr$340, int pc$342, unsigned int dst$344, unsigned char op$346)
 {
   unsigned char opcode_st;
-  unsigned char *addr_ptr$340;
-  _Bool is_null$342;
-  unsigned char *addr_ptr$344;
-  _Bool is_null$346;
-  unsigned char *addr_ptr$348;
-  _Bool is_null$350;
-  unsigned char *addr_ptr$352;
-  _Bool is_null$354;
-  opcode_st = get_opcode_mem_st_imm(op$336);
+  unsigned char *addr_ptr$350;
+  _Bool is_null$352;
+  unsigned char *addr_ptr$354;
+  _Bool is_null$356;
+  unsigned char *addr_ptr$358;
+  _Bool is_null$360;
+  unsigned char *addr_ptr$362;
+  _Bool is_null$364;
+  opcode_st = get_opcode_mem_st_imm(op$346);
   switch (opcode_st) {
     case 98:
-      addr_ptr$340 = check_mem(2U, 4U, addr$330);
-      is_null$342 = cmp_ptr32_nullM(addr_ptr$340);
-      if (is_null$342) {
+      addr_ptr$350 = check_mem(2U, 4U, addr$340);
+      is_null$352 = cmp_ptr32_nullM(addr_ptr$350);
+      if (is_null$352) {
         upd_flag(-2);
         return;
       } else {
-        store_mem_imm(4U, addr_ptr$340, imm$328);
+        store_mem_imm(4U, addr_ptr$350, imm$338);
         return;
       }
     case 106:
-      addr_ptr$344 = check_mem(2U, 2U, addr$330);
-      is_null$346 = cmp_ptr32_nullM(addr_ptr$344);
-      if (is_null$346) {
+      addr_ptr$354 = check_mem(2U, 2U, addr$340);
+      is_null$356 = cmp_ptr32_nullM(addr_ptr$354);
+      if (is_null$356) {
         upd_flag(-2);
         return;
       } else {
-        store_mem_imm(2U, addr_ptr$344, imm$328);
+        store_mem_imm(2U, addr_ptr$354, imm$338);
         return;
       }
     case 114:
-      addr_ptr$348 = check_mem(2U, 1U, addr$330);
-      is_null$350 = cmp_ptr32_nullM(addr_ptr$348);
-      if (is_null$350) {
+      addr_ptr$358 = check_mem(2U, 1U, addr$340);
+      is_null$360 = cmp_ptr32_nullM(addr_ptr$358);
+      if (is_null$360) {
         upd_flag(-2);
         return;
       } else {
-        store_mem_imm(1U, addr_ptr$348, imm$328);
+        store_mem_imm(1U, addr_ptr$358, imm$338);
         return;
       }
     case 122:
-      addr_ptr$352 = check_mem(2U, 8U, addr$330);
-      is_null$354 = cmp_ptr32_nullM(addr_ptr$352);
-      if (is_null$354) {
+      addr_ptr$362 = check_mem(2U, 8U, addr$340);
+      is_null$364 = cmp_ptr32_nullM(addr_ptr$362);
+      if (is_null$364) {
         upd_flag(-2);
         return;
       } else {
-        store_mem_imm(8U, addr_ptr$352, imm$328);
+        store_mem_imm(8U, addr_ptr$362, imm$338);
         return;
       }
     default:
@@ -786,57 +809,57 @@ void step_opcode_mem_st_imm(int imm$328, unsigned int addr$330, int pc$332, unsi
   }
 }
 
-void step_opcode_mem_st_reg(unsigned long long src64$356, unsigned int addr$358, int pc$360, unsigned int dst$362, unsigned char op$364)
+void step_opcode_mem_st_reg(unsigned long long src64$366, unsigned int addr$368, int pc$370, unsigned int dst$372, unsigned char op$374)
 {
-  unsigned char opcode_st$366;
-  unsigned char *addr_ptr$368;
-  _Bool is_null$370;
-  unsigned char *addr_ptr$372;
-  _Bool is_null$374;
-  unsigned char *addr_ptr$376;
-  _Bool is_null$378;
-  unsigned char *addr_ptr$380;
-  _Bool is_null$382;
-  opcode_st$366 = get_opcode_mem_st_reg(op$364);
-  switch (opcode_st$366) {
+  unsigned char opcode_st$376;
+  unsigned char *addr_ptr$378;
+  _Bool is_null$380;
+  unsigned char *addr_ptr$382;
+  _Bool is_null$384;
+  unsigned char *addr_ptr$386;
+  _Bool is_null$388;
+  unsigned char *addr_ptr$390;
+  _Bool is_null$392;
+  opcode_st$376 = get_opcode_mem_st_reg(op$374);
+  switch (opcode_st$376) {
     case 99:
-      addr_ptr$368 = check_mem(2U, 4U, addr$358);
-      is_null$370 = cmp_ptr32_nullM(addr_ptr$368);
-      if (is_null$370) {
+      addr_ptr$378 = check_mem(2U, 4U, addr$368);
+      is_null$380 = cmp_ptr32_nullM(addr_ptr$378);
+      if (is_null$380) {
         upd_flag(-2);
         return;
       } else {
-        store_mem_reg(4U, addr_ptr$368, src64$356);
+        store_mem_reg(4U, addr_ptr$378, src64$366);
         return;
       }
     case 107:
-      addr_ptr$372 = check_mem(2U, 2U, addr$358);
-      is_null$374 = cmp_ptr32_nullM(addr_ptr$372);
-      if (is_null$374) {
+      addr_ptr$382 = check_mem(2U, 2U, addr$368);
+      is_null$384 = cmp_ptr32_nullM(addr_ptr$382);
+      if (is_null$384) {
         upd_flag(-2);
         return;
       } else {
-        store_mem_reg(2U, addr_ptr$372, src64$356);
+        store_mem_reg(2U, addr_ptr$382, src64$366);
         return;
       }
     case 115:
-      addr_ptr$376 = check_mem(2U, 1U, addr$358);
-      is_null$378 = cmp_ptr32_nullM(addr_ptr$376);
-      if (is_null$378) {
+      addr_ptr$386 = check_mem(2U, 1U, addr$368);
+      is_null$388 = cmp_ptr32_nullM(addr_ptr$386);
+      if (is_null$388) {
         upd_flag(-2);
         return;
       } else {
-        store_mem_reg(1U, addr_ptr$376, src64$356);
+        store_mem_reg(1U, addr_ptr$386, src64$366);
         return;
       }
     case 123:
-      addr_ptr$380 = check_mem(2U, 8U, addr$358);
-      is_null$382 = cmp_ptr32_nullM(addr_ptr$380);
-      if (is_null$382) {
+      addr_ptr$390 = check_mem(2U, 8U, addr$368);
+      is_null$392 = cmp_ptr32_nullM(addr_ptr$390);
+      if (is_null$392) {
         upd_flag(-2);
         return;
       } else {
-        store_mem_reg(8U, addr_ptr$380, src64$356);
+        store_mem_reg(8U, addr_ptr$390, src64$366);
         return;
       }
     default:
@@ -848,81 +871,81 @@ void step_opcode_mem_st_reg(unsigned long long src64$356, unsigned int addr$358,
 
 void step(void)
 {
-  int pc$384;
-  unsigned long long ins$386;
-  unsigned char op$388;
+  int pc$394;
+  unsigned long long ins$396;
+  unsigned char op$398;
   unsigned char opc;
-  unsigned int dst$392;
-  unsigned long long dst64$394;
-  unsigned long long src64$396;
-  unsigned long long dst64$398;
-  unsigned int dst32$400;
-  unsigned int src32$402;
+  unsigned int dst$402;
   unsigned long long dst64$404;
-  int ofs$406;
-  unsigned long long src64$408;
-  int imm$410;
-  unsigned int src$412;
-  unsigned long long src64$414;
+  unsigned long long src64$406;
+  unsigned long long dst64$408;
+  unsigned int dst32$410;
+  unsigned int src32$412;
+  unsigned long long dst64$414;
   int ofs$416;
-  unsigned int addr$418;
-  unsigned long long dst64$420;
-  int ofs$422;
-  int imm$424;
-  unsigned int addr$426;
-  unsigned long long dst64$428;
-  unsigned int src$430;
-  unsigned long long src64$432;
-  int ofs$434;
+  unsigned long long src64$418;
+  int imm$420;
+  unsigned int src$422;
+  unsigned long long src64$424;
+  int ofs$426;
+  unsigned int addr$428;
+  unsigned long long dst64$430;
+  int ofs$432;
+  int imm$434;
   unsigned int addr$436;
-  pc$384 = eval_pc();
-  ins$386 = eval_ins(pc$384);
-  op$388 = get_opcode_ins(ins$386);
-  opc = get_opcode(op$388);
-  dst$392 = get_dst(ins$386);
+  unsigned long long dst64$438;
+  unsigned int src$440;
+  unsigned long long src64$442;
+  int ofs$444;
+  unsigned int addr$446;
+  pc$394 = eval_pc();
+  ins$396 = eval_ins(pc$394);
+  op$398 = get_opcode_ins(ins$396);
+  opc = get_opcode(op$398);
+  dst$402 = get_dst(ins$396);
   switch (opc) {
     case 7:
-      dst64$394 = eval_reg(dst$392);
-      src64$396 = get_src64(op$388, ins$386);
-      step_opcode_alu64(dst64$394, src64$396, dst$392, op$388);
+      dst64$404 = eval_reg(dst$402);
+      src64$406 = get_src64(op$398, ins$396);
+      step_opcode_alu64(dst64$404, src64$406, dst$402, op$398);
       return;
     case 4:
-      dst64$398 = eval_reg(dst$392);
-      dst32$400 = reg64_to_reg32(dst64$398);
-      src32$402 = get_src32(op$388, ins$386);
-      step_opcode_alu32(dst32$400, src32$402, dst$392, op$388);
+      dst64$408 = eval_reg(dst$402);
+      dst32$410 = reg64_to_reg32(dst64$408);
+      src32$412 = get_src32(op$398, ins$396);
+      step_opcode_alu32(dst32$410, src32$412, dst$402, op$398);
       return;
     case 5:
-      dst64$404 = eval_reg(dst$392);
-      ofs$406 = get_offset(ins$386);
-      src64$408 = get_src64(op$388, ins$386);
-      step_opcode_branch(dst64$404, src64$408, pc$384, ofs$406, op$388);
+      dst64$414 = eval_reg(dst$402);
+      ofs$416 = get_offset(ins$396);
+      src64$418 = get_src64(op$398, ins$396);
+      step_opcode_branch(dst64$414, src64$418, pc$394, ofs$416, op$398);
       return;
     case 0:
-      imm$410 = get_immediate(ins$386);
-      step_opcode_mem_ld_imm(imm$410, pc$384, dst$392, op$388);
+      imm$420 = get_immediate(ins$396);
+      step_opcode_mem_ld_imm(imm$420, pc$394, dst$402, op$398);
       return;
     case 1:
-      src$412 = get_src(ins$386);
-      src64$414 = eval_reg(src$412);
-      ofs$416 = get_offset(ins$386);
-      addr$418 = get_addr_ofs(src64$414, ofs$416);
-      step_opcode_mem_ld_reg(addr$418, pc$384, dst$392, op$388);
+      src$422 = get_src(ins$396);
+      src64$424 = eval_reg(src$422);
+      ofs$426 = get_offset(ins$396);
+      addr$428 = get_addr_ofs(src64$424, ofs$426);
+      step_opcode_mem_ld_reg(addr$428, pc$394, dst$402, op$398);
       return;
     case 2:
-      dst64$420 = eval_reg(dst$392);
-      ofs$422 = get_offset(ins$386);
-      imm$424 = get_immediate(ins$386);
-      addr$426 = get_addr_ofs(dst64$420, ofs$422);
-      step_opcode_mem_st_imm(imm$424, addr$426, pc$384, dst$392, op$388);
+      dst64$430 = eval_reg(dst$402);
+      ofs$432 = get_offset(ins$396);
+      imm$434 = get_immediate(ins$396);
+      addr$436 = get_addr_ofs(dst64$430, ofs$432);
+      step_opcode_mem_st_imm(imm$434, addr$436, pc$394, dst$402, op$398);
       return;
     case 3:
-      dst64$428 = eval_reg(dst$392);
-      src$430 = get_src(ins$386);
-      src64$432 = eval_reg(src$430);
-      ofs$434 = get_offset(ins$386);
-      addr$436 = get_addr_ofs(dst64$428, ofs$434);
-      step_opcode_mem_st_reg(src64$432, addr$436, pc$384, dst$392, op$388);
+      dst64$438 = eval_reg(dst$402);
+      src$440 = get_src(ins$396);
+      src64$442 = eval_reg(src$440);
+      ofs$444 = get_offset(ins$396);
+      addr$446 = get_addr_ofs(dst64$438, ofs$444);
+      step_opcode_mem_st_reg(src64$442, addr$446, pc$394, dst$402, op$398);
       return;
     default:
       upd_flag(-1);
@@ -934,17 +957,17 @@ void step(void)
 void bpf_interpreter_aux(unsigned int fuel)
 {
   unsigned int fuel0;
-  int len$442;
-  int pc$444;
+  int len$452;
+  int pc$454;
   int f;
   if (fuel == 0U) {
     upd_flag(-5);
     return;
   } else {
     fuel0 = fuel - 1U;
-    len$442 = eval_ins_len();
-    pc$444 = eval_pc();
-    if (0U <= pc$444 && pc$444 < len$442) {
+    len$452 = eval_ins_len();
+    pc$454 = eval_pc();
+    if (0U <= pc$454 && pc$454 < len$452) {
       step();
       f = eval_flag();
       if (f == 0) {
@@ -961,17 +984,17 @@ void bpf_interpreter_aux(unsigned int fuel)
   }
 }
 
-unsigned long long bpf_interpreter(unsigned int fuel$448)
+unsigned long long bpf_interpreter(unsigned int fuel$458)
 {
-  struct memory_region *mrs$450;
+  struct memory_region *mrs$460;
   struct memory_region *bpf_ctx;
-  int f$454;
-  mrs$450 = eval_mrs_regions();
-  bpf_ctx = get_mem_region(0U, mrs$450);
+  int f$464;
+  mrs$460 = eval_mrs_regions();
+  bpf_ctx = get_mem_region(0U, mrs$460);
   upd_reg(1U, (*bpf_ctx).start_addr);
-  bpf_interpreter_aux(fuel$448);
-  f$454 = eval_flag();
-  if (f$454 == 1) {
+  bpf_interpreter_aux(fuel$458);
+  f$464 = eval_flag();
+  if (f$464 == 1) {
     return eval_reg(0U);
   } else {
     return 0LLU;
