comm/Monad.v
@@ -65,3 +65,25 @@ Notation "'do' x <- a ; b" :=
   (bindM a (fun x => b))
     (at level 200, x name, a at level 100, b at level 200)
   : monad_scope.
+
+(* Given the immediate of the call, it returns a function pointer *)
+
+(* Let assume there is a bpf context pointer in the memory. For the time being, your interpreter does not use it.
+   Let keep it that way -- at least for the moment. *)
+Axiom _bpf_get_call : val -> M val. (**r here is Vint -> Vptr *)
+Axiom exec_function : val -> M val. (**r Vptr -> Vint *)
+Axiom lemma_bpf_get_call :
+  forall i st1,
+    exists ptr,
+      _bpf_get_call (Vint i) st1 = Some (ptr, st1) /\
+      (ptr = Vnullptr \/ (exists b ofs, ptr = Vptr b ofs)).
+Axiom lemma_exec_function0 :
+  forall b ofs st1,
+      exists v st2, exec_function (Vptr b ofs) st1 = Some (Vint v, st2) /\ cmp_ptr32_null (State.eval_mem st1) (Vptr b ofs) = Some false.
+(*
+Axiom lemma_exec_function1 :
+  forall st1, exec_function Vnullptr st1 = None. *)
+(*
+Axiom lemma_exec_function: forall (st:state) (i: int) (m:mem),
+      exec_function st (_bpf_get_call i) Vnullptr = NormalState (upd_pc (pc st) st) m.
+*)
