equivalence/switch.v
@@ -183,6 +183,9 @@ Definition get_instruction_if (opcode:nat) (rd rs:reg) (ofs: int) (i: int): inst
   else if opcode =? 0xdd then
     BPF_JUMP (Le Signed)   rd (inl rs) ofs
 
+  else if opcode =? 0x85 then
+    BPF_CALL i
+
   else if opcode =? 0x95 then
     BPF_RET
 
@@ -209,27 +212,7 @@ Lemma switch_if_same :
     get_instruction opcode rd rs ofs i = get_instruction_if opcode rd rs ofs i.
 Proof.
   intros.
-  unfold get_instruction, get_instruction_if. (*
-  Check Nat.eqb_eq.
-  match goal with
-  | |- ?A = ?B => apply Nat.eqb_eq with (n:= A) (m:=B)
-  end.
-  apply Nat.eqb_eq.
-  match goal with
-  | |- ?A = true => set (P := A)
-  end.
-  pattern (Nat.land op 240) in P.
-  match goal with
-  | P := ?F (Nat.land op 240) |- _=>
-      apply (Forall_exec_spec F 240)
-  end.
-  destruct (op =? 135).
-  vm_compute.
-  reflexivity.
-  vm_compute.
-  reflexivity.
-  rewrite Nat.land_comm.
-  apply land_bound.*)
+  unfold get_instruction, get_instruction_if.
 
   do 100 (destruct opcode; [reflexivity | idtac]).
   do 121 (destruct opcode; [reflexivity | idtac]).
@@ -326,6 +309,7 @@ Lemma switch_to_if :
 (Hsltr : Hopcode <> 205)
 (Hslei : Hopcode <> 213)
 (Hsler : Hopcode <> 221)
+(Hcall : Hopcode <> 133)
 (Hret : Hopcode <> 149),
   get_instruction Hopcode rd rs ofs i = BPF_ERR.
 Proof.
