src/DxInstructions.v
@@ -319,6 +319,18 @@ Definition step_opcode_branch (dst64: val64_t) (src64: val64_t) (pc: sint32_t) (
     else
       returnM tt
 
+  | op_BPF_CALL =>
+    if Nat.eqb op nat8_0x85 then
+      do f_ptr    <-- _bpf_get_call (val_intsoflongu src64);
+      do is_null  <-- cmp_ptr32_nullM f_ptr;
+        if is_null then
+          upd_flag BPF_ILLEGAL_CALL
+        else
+          do res  <-- exec_function f_ptr;
+            upd_reg R0 (Val.longofintu res)
+    else
+      do _ <-- upd_flag BPF_ILLEGAL_INSTRUCTION; returnM tt
+
   | op_BPF_RET => 
     if Nat.eqb op nat8_0x95 then
       do _ <-- upd_flag BPF_SUCC_RETURN; returnM tt
