src/DxNat.v
@@ -43,6 +43,7 @@ Definition nat8_zero := 0x00.
 Definition nat8_0x05 := 0x05.
 Definition nat8_0x84 := 0x84.
 Definition nat8_0x87 := 0x87.
+Definition nat8_0x85 := 0x85.
 Definition nat8_0x95 := 0x95.
 
 Definition nat8CompilableType :=
@@ -73,6 +74,9 @@ Definition C_NAT8_0x84: Csyntax.expr :=
 Definition C_NAT8_0x87: Csyntax.expr :=
   Csyntax.Eval (Vint (Int.repr (Z.of_nat nat8_0x87))) C_U8.
 
+Definition C_NAT8_0x85: Csyntax.expr :=
+  Csyntax.Eval (Vint (Int.repr (Z.of_nat nat8_0x85))) C_U8.
+
 Definition C_NAT8_0x95: Csyntax.expr :=
   Csyntax.Eval (Vint (Int.repr (Z.of_nat nat8_0x95))) C_U8.
 
@@ -89,6 +93,7 @@ Definition Const_nat8_zero := constant nat8SymbolType nat8_zero C_NAT8_0x00.
 Definition Const_nat8_0x05 := constant nat8SymbolType nat8_0x05 C_NAT8_0x05.
 Definition Const_nat8_0x84 := constant nat8SymbolType nat8_0x84 C_NAT8_0x84.
 Definition Const_nat8_0x87 := constant nat8SymbolType nat8_0x87 C_NAT8_0x87.
+Definition Const_nat8_0x85 := constant nat8SymbolType nat8_0x85 C_NAT8_0x85.
 Definition Const_nat8_0x95 := constant nat8SymbolType nat8_0x95 C_NAT8_0x95.
 
 Definition nat8Tonat8ToboolSymbolType :=
@@ -131,5 +136,6 @@ Module Exports.
   Definition Const_nat8_0x05    := Const_nat8_0x05.
   Definition Const_nat8_0x84    := Const_nat8_0x84.
   Definition Const_nat8_0x87    := Const_nat8_0x87.
+  Definition Const_nat8_0x85    := Const_nat8_0x85.
   Definition Const_nat8_0x95    := Const_nat8_0x95.
 End Exports.
